theories/Program.v
@@ -20,6 +20,7 @@ Require Import Coq.Program.Tactics.
 Require Import Coq.Relations.Relations.
 Require Import Coq.Setoids.Setoid.
 Require Import Coq.Program.Basics.
+Require Import Coq.Logic.FunctionalExtensionality.
 
 Require Import FreeSpec.Semantics.
 
@@ -69,16 +70,13 @@ Inductive Program
           (A:  Type) :=
 | Pure (a:  A)
   : Program I A
-| Request (e:  I A)
-  : Program I A
-| Bind {B:  Type}
-       (p:  Program I B)
-       (f:  B -> Program I A)
+| Request {B:  Type}
+          (e:  I B)
+          (f:  B -> Program I A)
   : Program I A.
 
 Arguments Pure [I A] (a).
-Arguments Request [I A] (e).
-Arguments Bind [I A B] (p f).
+Arguments Request [I A B] (e f).
 
 (** ** Realisation
 
@@ -97,10 +95,8 @@ Fixpoint runProgram
   match p with
   | Pure a
     => (a, sig)
-  | Request e
-    => handle sig e
-  | Bind q f
-    => runProgram (snd (runProgram sig q)) (f (fst (runProgram sig q)))
+  | Request e f
+    => runProgram (snd (handle sig e)) (f (fst (handle sig e)))
   end.
 
 Definition evalProgram
@@ -127,51 +123,11 @@ Definition execProgram
 
  *)
 
-Inductive program_eq
-          {I:  Type -> Type}
-          {A:  Type}
-  : Program I A -> Program I A -> Prop :=
-| program_eq_refl (p:  Program I A)
-  : program_eq p p
-| program_eq_sym (p q:  Program I A)
-                  (H:    program_eq p q)
-  : program_eq q p
-| program_eq_trans (p q r:  Program I A)
-                    (Hpq:   program_eq p q)
-                    (Hqr:   program_eq q r)
-  : program_eq p r
-| program_eq_append_pure (p:  Program I A)
-  : program_eq p (Bind p (@Pure I A))
-| program_eq_bind_ret {B:  Type}
-                       (x:  B)
-                       (f:  B -> Program I A)
-  : program_eq (Bind (Pure x) f) (f x)
-| program_eq_bind_assoc {B C:  Type}
-                         (p:   Program I B)
-                         (f:   B -> Program I C)
-                         (g:   C -> Program I A)
-  : program_eq (Bind (Bind p f) g) (Bind p (fun x => Bind (f x) g))
-| program_eq_bind {B:    Type}
-                   (p q:  Program I B)
-                   (f g:  B -> Program I A)
-                   (Hpq:  @program_eq I B p q)
-                   (Hfg:  forall (x:  B), program_eq (f x) (g x))
-  : program_eq (Bind p f) (Bind q g).
-
-Add Parametric Relation
-    (I:  Interface)
-    (A:  Type)
-  : (Program I A) (program_eq)
-    reflexivity  proved by program_eq_refl
-    symmetry     proved by program_eq_sym
-    transitivity proved by program_eq_trans
-      as program_equiv.
-
 Instance program_Eq
          (I:  Interface)
          (A:  Type)
   : Equality (Program I A) :=
-  { equal := program_eq
+  { equal := eq
   }.
 
 (** Also, we can easily show the [program_eq] property is strong
@@ -180,114 +136,31 @@ Instance program_Eq
 
  *)
 
-Lemma run_program_bind_assoc
-      {I:    Interface}
-      {A B:  Type}
-      (sig:  Semantics I)
-      (p:    Program I A)
-      (f:    A -> Program I B)
-  : runProgram sig (Bind p f)
-    == runProgram (execProgram sig p) (f (evalProgram sig p)).
-Proof.
-  reflexivity.
-Qed.
-
-Lemma eval_program_bind_assoc
-      {I:    Interface}
-      {A B:  Type}
-      (sig:  Semantics I)
-      (p:    Program I A)
-      (f:    A -> Program I B)
-  : evalProgram sig (Bind p f)
-    = evalProgram (execProgram sig p) (f (evalProgram sig p)).
-Proof.
-  reflexivity.
-Qed.
-
-Lemma exec_program_bind_assoc
-      {I:    Interface}
-      {A B:  Type}
-      (sig:  Semantics I)
-      (p:    Program I A)
-      (f:    A -> Program I B)
-  : execProgram sig (Bind p f)
-    = execProgram (execProgram sig p) (f (evalProgram sig p)).
-Proof.
-  reflexivity.
-Qed.
-
 Add Parametric Morphism
     (I: Interface)
     (A: Type)
   : (runProgram)
-    with signature (@semantics_eq I) ==> eq ==> (@run_semantics_eq I A)
+    with signature (@semantics_eq I) ==> (@equal (Program I A) _) ==> (@run_semantics_eq I A)
   as run_program_morphism_2.
 Proof.
-  intros sig1 sig2 Heq_sig p.
+  intros sig1 sig2 Heq_sig p q Heq_p.
+  induction Heq_p.
   revert sig1 sig2 Heq_sig.
   induction p; intros sig1 sig2 Heq_sig.
   + constructor; [ reflexivity |].
     apply Heq_sig.
-  + constructor; apply Heq_sig.
-  + repeat rewrite run_program_bind_assoc.
-    assert (rw:  evalProgram sig1 p = evalProgram sig2 p). {
-      apply IHp.
-      exact Heq_sig.
-    }
-    rewrite rw.
+  + cbn.
+    assert (Hx: fst (handle sig1 e) = fst (handle sig2 e)) by apply Heq_sig.
+    rewrite Hx.
     apply H.
-    apply IHp.
-    exact Heq_sig.
-Qed.
-
-Add Parametric Morphism
-    (I:  Interface)
-    (A:  Type)
-  : (runProgram)
-    with signature eq ==> (@equal (Program I A) _) ==> (@run_semantics_eq I A)
-  as run_program_morphism_1.
-Proof.
-  intros sig p q Heq.
-  revert sig.
-  induction Heq; intros sig.
-  + reflexivity.
-  + symmetry.
-    apply (IHHeq sig).
-  + etransitivity; [ apply (IHHeq1 sig)
-                   | apply (IHHeq2 sig)
-                   ].
-  + constructor; reflexivity.
-  + constructor; reflexivity.
-  + constructor; reflexivity.
-  + repeat rewrite run_program_bind_assoc.
-    assert (Hstep: run_semantics_eq (runProgram sig p) (runProgram sig q))
-      by apply IHHeq.
-    assert (rw:  execProgram sig p == execProgram sig q) by apply Hstep.
-    assert (rw': evalProgram sig p = evalProgram sig q) by apply Hstep.
-    rewrite rw.
-    rewrite rw'.
-    apply H.
-Qed.
-
-Add Parametric Morphism
-    (I:  Interface)
-    (A:  Type)
-  : (evalProgram)
-    with signature (@equal (Semantics I) _) ==> (@program_eq I A) ==> (eq)
-  as eval_program_morphism.
-Proof.
-  intros sig sig' Heqs p q Heqp.
-  unfold evalProgram.
-  rewrite Heqs.
-  rewrite Heqp.
-  reflexivity.
+    apply Heq_sig.
 Qed.
 
 Add Parametric Morphism
     (I:  Interface)
     (A:  Type)
   : (execProgram)
-    with signature (@equal (Semantics I) _) ==> (@program_eq I A) ==> (@semantics_eq I)
+    with signature (@equal (Semantics I) _) ==> (@equal (Program I A) _) ==> (@semantics_eq I)
   as exec_program_morphism.
 Proof.
   intros sig sig' Heqs p q Heqp.
@@ -298,22 +171,17 @@ Proof.
 Qed.
 
 Add Parametric Morphism
-    (I:    Interface)
-    (A B:  Type)
-  : (@Bind I B A)
-    with signature (@equal (Program I A) _)
-                     ==> (@equal (A -> Program I B) _)
-                     ==> (@equal (Program I B) _)
-      as pbind_morphism.
+    (I:  Interface)
+    (A:  Type)
+  : (evalProgram)
+    with signature (@equal (Semantics I) _) ==> (@equal (Program I A) _) ==> eq
+  as eval_program_morphism.
 Proof.
-  intros p q Heq f g Heq_f.
-  constructor.
-  apply program_eq_bind.
-  + symmetry.
-    exact Heq.
-  + intros x.
-    symmetry.
-    apply Heq_f.
+  intros sig sig' Heqs p q Heqp.
+  unfold evalProgram.
+  rewrite Heqs.
+  rewrite Heqp.
+  reflexivity.
 Qed.
 
 Lemma program_eq_sig_eq
@@ -361,13 +229,95 @@ Qed.
 
  *)
 
+Fixpoint pbind
+         {I:    Interface}
+         {A B:  Type}
+         (p:    Program I A)
+         (f:    A -> Program I B)
+  : Program I B :=
+  match p with
+  | Pure x => f x
+  | Request e g => Request e (fun x => pbind (g x) f)
+  end.
+
+Lemma run_program_bind_assoc
+      {I:    Interface}
+      {A B:  Type}
+      (sig:  Semantics I)
+      (p:    Program I A)
+      (f:    A -> Program I B)
+  : runProgram sig (pbind p f)
+    == runProgram (execProgram sig p) (f (evalProgram sig p)).
+Proof.
+  revert sig; induction p; intro sig.
+  + reflexivity.
+  + apply H.
+Qed.
+
+Lemma eval_program_bind_assoc
+      {I:    Interface}
+      {A B:  Type}
+      (sig:  Semantics I)
+      (p:    Program I A)
+      (f:    A -> Program I B)
+  : evalProgram sig (pbind p f)
+    = evalProgram (execProgram sig p) (f (evalProgram sig p)).
+Proof.
+  unfold evalProgram.
+  rewrite run_program_bind_assoc.
+  reflexivity.
+Qed.
+
+Lemma exec_program_bind_assoc
+      {I:    Interface}
+      {A B:  Type}
+      (sig:  Semantics I)
+      (p:    Program I A)
+      (f:    A -> Program I B)
+  : execProgram sig (pbind p f)
+    = execProgram (execProgram sig p) (f (evalProgram sig p)).
+Proof.
+  revert sig; induction p; intro sig.
+  + reflexivity.
+  + apply H.
+Qed.
+
+Lemma program_eq_append_pure
+      {I:  Type -> Type}
+      {A:  Type}
+      (p:  Program I A)
+  : p = pbind p (@Pure I A).
+Proof.
+  induction p.
+  + reflexivity.
+  + cbn.
+    apply functional_extensionality in H.
+    rewrite <- H.
+    reflexivity.
+Qed.
+
+Lemma program_eq_bind_assoc
+      {I:      Type -> Type}
+      {A B C:  Type}
+      (p:      Program I A)
+      (f:      A -> Program I B)
+      (g:      B -> Program I C)
+  : pbind (pbind p f) g = pbind p (fun x => pbind (f x) g).
+Proof.
+  induction p; [reflexivity |].
+  cbn.
+  apply functional_extensionality in H.
+  rewrite H.
+  reflexivity.
+Qed.
+
 Definition program_map
            {I:    Interface}
            {A B:  Type}
            (f:    A -> B)
            (p:    Program I A)
   : Program I B :=
-  Bind p (fun x => Pure (f x)).
+  pbind p (fun x => Pure (f x)).
 
 Instance program_Functor
          (I:  Interface)
@@ -383,9 +333,6 @@ Proof.
     unfold compose.
     unfold program_map.
     rewrite program_eq_bind_assoc.
-    apply program_eq_bind; [ reflexivity |].
-    intros y.
-    rewrite program_eq_bind_ret.
     reflexivity.
 Defined.
 
@@ -395,13 +342,24 @@ Definition program_apply
            (pf:   Program I (A -> B))
            (p:    Program I A)
   : Program I B :=
-  Bind pf (fun f => Bind p (fun x => Pure (f x))).
+  pbind pf (fun f => pbind p (fun x => Pure (f x))).
 
 Definition program_pure
            {I:  Interface}
            {A:  Type}
   : A -> Program I A :=
   @Pure I A.
+
+Lemma program_eq_bind
+      {I:    Type -> Type}
+      {A B:  Type}
+      (p:    Program I A)
+      (f g:  A -> Program I B)
+  : f = g -> pbind p f = pbind p g.
+Proof.
+  intros R; rewrite R.
+  reflexivity.
+Qed.
 
 Instance program_Applicative
          (I:  Interface)
@@ -412,74 +370,54 @@ Instance program_Applicative
 Proof.
   + intros A HA p.
     unfold program_apply, program_pure.
-    rewrite program_eq_bind_ret.
+    cbn.
     rewrite <- program_eq_append_pure.
     reflexivity.
   + intros A B C HC u v p.
     unfold program_apply, program_pure.
-    rewrite program_eq_bind_ret.
-    repeat rewrite program_eq_bind_assoc.
-    apply program_eq_bind; [ reflexivity |].
-    intros x.
-    rewrite program_eq_bind_ret.
-    repeat rewrite program_eq_bind_assoc.
-    apply program_eq_bind; [ reflexivity |].
-    intros y.
-    unfold compose.
-    rewrite program_eq_bind_ret.
-    repeat rewrite program_eq_bind_assoc.
-    apply program_eq_bind; [ reflexivity |].
-    intros z.
-    rewrite program_eq_bind_ret.
-    reflexivity.
-  + intros A B HB v x.
-    unfold program_apply, program_pure.
-    repeat rewrite program_eq_bind_ret.
-    reflexivity.
-  + intros A B HA u y.
-    unfold program_apply, program_pure.
-    repeat rewrite program_eq_bind_ret.
-    apply program_eq_bind; [ reflexivity |].
-    intros x.
-    repeat rewrite program_eq_bind_ret.
-    reflexivity.
-  + intros A B HA g x.
     cbn.
-    unfold program_map, program_apply, program_pure.
-    rewrite program_eq_bind_ret.
-    apply program_eq_bind; [ reflexivity |].
+    repeat rewrite program_eq_bind_assoc.
+    cbn.
+    apply program_eq_bind.
+    apply functional_extensionality.
+    intros x.
+    repeat rewrite program_eq_bind_assoc.
+    apply program_eq_bind.
+    apply functional_extensionality.
+    intros y.
+    cbn.
+    repeat rewrite program_eq_bind_assoc.
+    apply program_eq_bind.
+    apply functional_extensionality.
+    intros z.
     reflexivity.
+  + reflexivity.
+  + reflexivity.
+  + reflexivity.
 Defined.
-
-Definition program_bind
-           {I:    Interface}
-           {A B:  Type}
-  : Program I A -> (A -> Program I B) -> Program I B :=
-  @Bind I B A.
 
 Instance program_Monad
          (I:  Interface)
   : Monad (Program I) :=
-  { bind := @program_bind I
+  { bind := @pbind I
   }.
 Proof.
-  + intros A B HB x f.
-    apply program_eq_bind_ret.
-  + intros A HA x.
-    unfold program_bind.
+  + reflexivity.
+  + intros A Ha p.
+    cbn.
     rewrite <- program_eq_append_pure.
     reflexivity.
-  + intros A B C HC f g h.
-    unfold program_bind.
-    apply program_eq_bind_assoc.
-  + intros A B HB x f g Heq.
-    rewrite Heq.
+  + intros A B C HC x f g.
+    rewrite program_eq_bind_assoc.
     reflexivity.
-  + intros A B HA x f.
+  + intros A B HB p f g Heq.
+    cbn in Heq.
+    unfold function_equal in Heq.
+    cbn in Heq.
+    apply program_eq_bind.
+    now apply functional_extensionality.
+  + intros A B HB p f.
     cbn.
-    unfold program_map, program_bind.
-    apply program_eq_bind; [ reflexivity |].
-    intros y.
     reflexivity.
 Defined.
 
@@ -505,10 +443,8 @@ Fixpoint runProgram'
   match p with
   | Pure a
     => (a, sig)
-  | Request e
-    => handle sig e
-  | Bind q f
-    => let o := runProgram' sig q
+  | Request e f
+    => let o := handle sig e
        in runProgram' (snd o) (f (fst o))
   end.
 
@@ -526,155 +462,11 @@ Fixpoint interface_map
          {I I':  Interface}
          {A:     Type}
          (p:     Program I A)
-         (map:   forall (A:  Type), I A -> I' A)
+         (map:   forall {A:  Type}, I A -> I' A)
   : Program I' A :=
   match p with
   | Pure x
     => Pure x
-  | Request e
-    => Request (map A e)
-  | Bind q f
-    => Bind (interface_map q map) (fun x => interface_map (f x) map)
+  | Request e f
+    => Request (map e) (fun x => interface_map (f x) (fun _ x => map x))
   end.
-
-Inductive View
-          (I:  Type -> Type)
-          (A:  Type)
-  : Type :=
-| Result (x:  A)
-  : View I A
-| Seq {B:    Type}
-      (eff:  I B)
-      (f:    B -> Program I A)
-  : View I A.
-
-Arguments Result {I A} (x).
-Arguments Seq {I A B} (eff f).
-
-Require Import FunInd.
-
-Function view
-         {I:  Type -> Type}
-         {A:  Type}
-         (p:  Program I A)
-  : View I A :=
-  match p with
-  | Pure x
-    => Result x
-  | Request eff
-    => Seq eff (@Pure I A)
-  | Bind p f
-    => match view p with
-       | Result x
-         => view (f x)
-       | Seq eff h
-         => Seq eff (fun x => Bind (h x) f)
-       end
-  end.
-
-Theorem program_eq'_eval_eq
-        {I:    Type -> Type}
-        {A:    Type}
-        (p q:  Program I A)
-  : p == q -> forall (sig:  Semantics I),
-      runProgram sig p = runProgram sig q.
-Proof.
-  intros Heq.
-  induction Heq; intros sig.
-  + reflexivity.
-  + symmetry.
-    apply IHHeq.
-  + transitivity (runProgram sig q).
-    ++ apply IHHeq1.
-    ++ apply IHHeq2.
-  + cbn.
-    destruct (runProgram sig p).
-    reflexivity.
-  + reflexivity.
-  + reflexivity.
-  + cbn.
-    rewrite IHHeq.
-    rewrite H.
-    reflexivity.
-Qed.
-
-Function simplify
-         {I:  Type -> Type}
-         {A:  Type}
-         (p:  Program I A)
-  : Program I A :=
-  match view p with
-  | Result x
-    => Pure x
-  | Seq eff f
-    => Bind (Request eff) f
-  end.
-
-Theorem simplify_eq
-        {I:  Type -> Type}
-        {A:  Type}
-        (p:  Program I A)
-  : p == (simplify p).
-Proof.
-  induction p.
-  + apply program_eq_refl.
-  + cbn.
-    apply program_eq_append_pure.
-  + assert ((simplify (Bind p f))
-            == (Bind (simplify p) (fun x => simplify (f x)))). {
-      functional induction (simplify p).
-      + unfold simplify.
-        cbn.
-        rewrite e.
-        fold (simplify (f x)).
-        eapply program_eq_trans.
-        apply program_eq_sym.
-        apply H.
-        apply program_eq_sym.
-        eapply program_eq_trans.
-        eapply program_eq_bind_ret.
-        fold (simplify (f x)).
-        apply program_eq_sym.
-        apply H.
-      + unfold simplify.
-        cbn.
-        rewrite e.
-        eapply program_eq_trans.
-        apply program_eq_sym.
-        apply program_eq_bind_assoc.
-        apply program_eq_bind.
-        apply program_eq_refl.
-        intros x.
-        fold (simplify (f x)).
-        apply H.
-    }
-    apply program_eq_trans with (q:=(Bind (simplify p) (fun x : B => simplify (f x)))).
-    ++ apply program_eq_bind.
-       apply IHp.
-       apply H.
-    ++ apply program_eq_sym.
-       apply H0.
-Qed.
-
-(* FIXME: not enough *)
-Theorem program_request_seq_ind
-        {I:       Type -> Type}
-        {A:       Type}
-        (P:       Program I A -> Prop)
-        (Hmorph:  forall (p q:  Program I A),
-            p == q -> (P p <-> P q))
-        (Hres:   forall (x:  A), P (Pure x))
-        (Hseq:   forall {B:    Type}
-                        (eff:  I B)
-                        (f:    B -> Program I A),
-            P (Bind (Request eff) f))
-  : forall (p:  Program I A),
-    P p.
-Proof.
-  intros p.
-  assert (Hsimp:  p == (simplify p)) by apply simplify_eq.
-  apply (Hmorph (simplify p) p (program_eq_sym _ _ Hsimp)).
-  functional induction (simplify p).
-  + apply Hres.
-  + apply Hseq.
-Qed.
